src/ocaml-output/FStar_Syntax_Util.ml
@@ -4767,17 +4767,15 @@ let (ctx_uvar_typ :
       FStar_Syntax_Unionfind.find_decoration
         u.FStar_Syntax_Syntax.ctx_uvar_head in
     uu___.FStar_Syntax_Syntax.uvar_decoration_typ
-let (ctx_uvar_uvar_kind :
+let (ctx_uvar_kind :
   FStar_Syntax_Syntax.ctx_uvar ->
-    (FStar_Syntax_Syntax.ctx_uvar FStar_Pervasives_Native.option,
-      FStar_Syntax_Syntax.term' FStar_Syntax_Syntax.syntax Prims.list)
+    (FStar_Syntax_Syntax.ctx_uvar FStar_Pervasives_Native.option, unit)
       FStar_Pervasives.either)
   =
   fun u ->
     let uu___ =
       FStar_Syntax_Unionfind.find_decoration
         u.FStar_Syntax_Syntax.ctx_uvar_head in
-    uu___.FStar_Syntax_Syntax.uvar_decoration_uvar_kind
+    uu___.FStar_Syntax_Syntax.uvar_decoration_kind
 let (is_guard_ctx_uvar : FStar_Syntax_Syntax.ctx_uvar -> Prims.bool) =
-  fun u ->
-    let uu___ = ctx_uvar_uvar_kind u in FStar_Pervasives.uu___is_Inr uu___
+  fun u -> let uu___ = ctx_uvar_kind u in FStar_Pervasives.uu___is_Inr uu___
