src/syntax/FStar.Syntax.Syntax.fsti
@@ -153,16 +153,16 @@ and ctx_uvar_meta_t =
 and ctx_uvar_and_subst = ctx_uvar * subst_ts
 
 //
-// kind:
+// u.kind:
 //   Inl None ==> This uvar typing guard is not to be accumulated in any other uvar,
-//   Inl (Some u) ==> This uvar's typing guard will be added to u,
-//                     u's kind must be Inr l
-//   Inr l ==> This uvar is only accumulating the typing guards for some uvars in l
+//   Inl (Some u') ==> This uvar's typing guard will be added to u',
+//                     u's kind must be Inr ()
+//   Inr () ==> This uvar is accumulating the typing guard for some uvar
 //
 and uvar_decoration = {
   uvar_decoration_typ:typ;
   uvar_decoration_should_check:should_check_uvar;
-  uvar_decoration_uvar_kind:either (option ctx_uvar) (list term);
+  uvar_decoration_kind:either (option ctx_uvar) unit
 }
 
 and uvar = Unionfind.p_uvar (option term * uvar_decoration) * version * Range.range
