src/syntax/FStar.Syntax.Util.fst
@@ -2407,7 +2407,7 @@ let ctx_uvar_should_check (u:ctx_uvar) =
 let ctx_uvar_typ (u:ctx_uvar) = 
   (Unionfind.find_decoration u.ctx_uvar_head).uvar_decoration_typ
 
-let ctx_uvar_uvar_kind (u:ctx_uvar) = 
-  (Unionfind.find_decoration u.ctx_uvar_head).uvar_decoration_uvar_kind
+let ctx_uvar_kind (u:ctx_uvar) = 
+  (Unionfind.find_decoration u.ctx_uvar_head).uvar_decoration_kind
 
-let is_guard_ctx_uvar (u:ctx_uvar) = Inr? (ctx_uvar_uvar_kind u)
+let is_guard_ctx_uvar (u:ctx_uvar) = Inr? (ctx_uvar_kind u)
