src/typechecker/FStar.TypeChecker.Rel.fsti
@@ -53,6 +53,10 @@ val solve_non_tactic_deferred_constraints: maybe_defer_flex_flex:bool -> env -> 
 val discharge_guard_no_smt    : env -> guard_t -> guard_t
 val discharge_guard           : env -> guard_t -> guard_t
 val force_trivial_guard       : env -> guard_t -> unit
+
+val core_check_and_maybe_add_to_guard_uvar:
+  env -> ctx_uvar -> term -> typ -> must_tot:bool -> Env.core_check_ret_t
+
 val is_implicit_resolved      : env -> Env.implicit -> bool
 val check_implicit_solution_for_tac : env -> Env.implicit -> option (term * typ)
 val resolve_implicits         : env -> guard_t -> guard_t
